Finish formalization of uniformize_fun

Escallon/Chomsky_Normal_Form_Fun/Chomsky_Normal_Form_Fun.thy
@@ -2,37 +2,243 @@ theory Chomsky_Normal_Form_Fun
   imports "Context_Free_Grammar.Chomsky_Normal_Form" HOL.List
 begin
 
-fun tm_list_of_prods :: "('n,'t) prods \<Rightarrow> ('n,'t) sym list" where
+fun tm_list_of_prods :: "('n,'t) prods \<Rightarrow> 't list" where
   "tm_list_of_prods ps = 
-    (let rs = map snd ps in filter isTm (concat rs))"
+    (let rs = map snd ps in map destTm (filter isTm (concat rs)))"
 
-lemma in_tm_list_of_prods_impl_Tm:
-  assumes "tm \<in> set (tm_list_of_prods ps)"
-  obtains t where "tm = Tm t"
+lemma tm_list_of_prods_is_tms:
+  "tm \<in> set (tm_list_of_prods ps) \<longleftrightarrow> tm \<in> tms ps"
 proof -
-  from assms obtain xs where "tm \<in> set (filter isTm xs)" by auto
-  then show thesis using that isTm_def by fastforce 
+  have "tm \<in> set (tm_list_of_prods ps) = 
+    (tm \<in> set (map destTm (filter isTm (concat (map snd ps)))))"
+    by force
+  also have "... = (Tm tm \<in> set (filter isTm (concat (map snd ps))))" 
+    using destTm_o_Tm
+    by (smt (verit, best) destTm.simps filter_set in_set_conv_nth isTm_def length_map member_filter
+        nth_map nth_mem)
+  also have "... = (tm \<in> (\<Union>(A,w)\<in>(set ps). tms_syms w))"
+    using tms_syms_def by fastforce
+  also have "... = (tm \<in> tms ps)" unfolding Tms_def by blast
+  finally show ?thesis .
 qed
 
-(*(l,r) as argument in f bad practice?*)
-fun uniformize_tm :: "['t, 'n, ('n,'t) prods] \<Rightarrow> ('n,'t) prods" where
-  "uniformize_tm t nt ps = 
-    (let f = (\<lambda>(l,r). if length r < 2 then (l,r) 
-                      else (l,map (\<lambda>s. if s = (Tm t) then (Nt nt) else s) r))  
-    in map f ps)"
+fun replace_tm :: "['t, 'n, ('n,'t) syms] \<Rightarrow> ('n,'t) syms" where
+  "replace_tm t A [] = []" |
+  "replace_tm t A (s # sms) = (if s = Tm t then Nt A # sms else s # replace_tm t A sms)"
 
-lemma uniformize_tm_is_uniformized:
-  "uniformize (fresh (nts ps \<union> {S})) t S ps (uniformize_tm t (fresh (nts ps \<union> {S})) ps)"
-  sorry
+lemma replace_tm_length_unchanged[simp]: 
+  "length (replace_tm t A sms) = length sms"
+  by (induction sms) auto
+  
+
+lemma replace_tm_id_iff_tm_notin_syms:
+  shows "Tm t \<notin> set sms \<longleftrightarrow> replace_tm t A sms = sms"
+  by (induction sms) auto
+
+(*Proofs break with iff lemma. Fix?*)
+lemma tm_notin_syms_impl_replace_tm_id:
+  assumes "Tm t \<notin> set sms" 
+  shows "replace_tm t A sms = sms"
+  using assms replace_tm_id_iff_tm_notin_syms by fast
+lemma replace_tm_id_impl_tm_notin_syms:
+  assumes "replace_tm t A sms = sms"
+  shows "Tm t \<notin> set sms"
+  using assms replace_tm_id_iff_tm_notin_syms by fast
+
+(*Strengthen with "Tm t \<notin> set p?*)
+lemma replace_tm_replaces_single:
+  assumes "replace_tm t A sms \<noteq> sms"
+  obtains p s where "sms = p@[Tm t]@s"
+                    "replace_tm t A sms = p@[Nt A]@s"
+using assms proof (induction sms arbitrary: thesis)
+  case (Cons s sms)
+  from Cons(3) have t_in_ssms: "Tm t \<in> set (s#sms)" using tm_notin_syms_impl_replace_tm_id by fast
+  consider (eq) "s = Tm t" | (neq) "s \<noteq> Tm t" by blast
+  then show ?case 
+  proof cases
+    case eq
+    then obtain p q where "s#sms = p@[Tm t]@q" "p = []" by auto
+    moreover from eq have "replace_tm t A (s#sms) = Nt A#sms" by simp
+    ultimately show thesis using Cons(2) by fastforce
+  next
+    case neq
+    with t_in_ssms have "Tm t \<in> set sms" 
+      by simp
+    with Cons(1) replace_tm_id_impl_tm_notin_syms 
+    obtain p q where pq_defs: "sms = p@[Tm t]@q" "replace_tm t A sms = p@[Nt A]@q" by metis
+    with neq have "replace_tm t A (s#sms) = (s#p)@[Nt A]@q" by auto
+    then show ?thesis using Cons(2) pq_defs by (meson Cons_eq_appendI)
+  qed
+qed simp
 
 
-fun uniformize' :: "['n::infinite, ('n,'t) syms, ('n,'t) prods] \<Rightarrow> ('n,'t) prods" where
-  "uniformize' _ [] ps = ps" |
-  "uniformize' S (t#ts) ps = 
-    uniformize' S ts (uniformize_tm (destTm t) (fresh (nts ps \<union> {S})) ps)"
+  
+(*Define separate uniformize_fun :: ['t, 'n, ('n,'t) prods] \<Rightarrow> ('n,'t) prods?*)
+fun uniformize_fun :: "['t, 'n, ('n,'t) prods, ('n,'t) prods] \<Rightarrow> ('n,'t) prods" where
+  "uniformize_fun _ _ ps0 [] = ps0" |
+  "uniformize_fun t A ps0 ((l,r) # ps) = 
+    (let r' = replace_tm t A r in 
+      if r = r' \<or> length r < 2 then uniformize_fun t A ps0 ps
+      else (removeAll (l,r) ps0) @ [(A, [Tm t]), (l,r')])" 
 
-fun uniformize_fun :: "['n::infinite, ('n,'t) prods] \<Rightarrow> ('n,'t) prods" where
-  "uniformize_fun S ps = uniformize' S (tm_list_of_prods ps) ps"
+lemma uniformize_fun_id:
+  assumes "\<forall>(l,r)\<in>set ps. Tm t \<notin> set r \<or> length r < 2"
+  shows "uniformize_fun t A ps0 ps = ps0"
+  using assms tm_notin_syms_impl_replace_tm_id by (induction ps) fastforce+
+
+lemma uniformize_fun_uniform_prepend:
+   "\<forall>(l,r)\<in>set xs. Tm t \<notin> set r \<or> length r < 2 \<Longrightarrow>
+    uniformize_fun t A ps0 (xs@ps) = uniformize_fun t A ps0 ps"
+proof (induction xs)
+  case (Cons x xs)
+  then obtain l r where lr_def: "x = (l,r)" by auto
+  hence "uniformize_fun t A ps0 ((x#xs)@ps) = uniformize_fun t A ps0 ((l,r)#xs@ps)" by simp
+  also have "... = uniformize_fun t A ps0 (xs@ps)"
+  proof -
+    from Cons(2) lr_def have "Tm t \<notin> set r \<or> length r < 2" by simp
+    hence "replace_tm t A r = r \<or> length r < 2" using tm_notin_syms_impl_replace_tm_id by fast
+    thus ?thesis by auto
+  qed
+  also have "... = uniformize_fun t A ps0 ps" using Cons by simp
+  finally show ?case .
+qed simp
+
+lemma uniformize_fun_ps0_app:
+  assumes "A = fresh (nts ps)"
+          "\<forall>(l,r)\<in>set xs. Tm t \<notin> set r \<or> length r < 2"
+  shows "uniformize_fun t A (xs@ys) ps = xs @ uniformize_fun t A ys ps"
+proof (induction ps)
+  case (Cons p ps)
+  then obtain l r where lr_def: "p = (l,r)" 
+    by fastforce
+  then consider (not_unif) "Tm t \<in> set r \<and> length r \<ge> 2" | (unif) "Tm t \<notin> set r \<or> length r < 2"
+    by linarith
+  then show ?case 
+  proof cases
+    case not_unif
+    with assms(2) lr_def have p_notin_xs: "p \<notin> set xs" by auto
+    from not_unif lr_def have "uniformize_fun t A (xs@ys) (p#ps) 
+                      = removeAll p (xs@ys) @ [(A, [Tm t]), (l,replace_tm t A r)]" 
+      by (smt (verit) replace_tm_id_iff_tm_notin_syms uniformize_fun.simps(2)
+          verit_comp_simplify1(3))
+    also have "... = xs @ removeAll p ys @ [(A, [Tm t]), (l,replace_tm t A r)]"
+      using p_notin_xs by simp
+    also have "... = xs @ uniformize_fun t A ys (p#ps)" using not_unif 
+      by (smt (verit) lr_def replace_tm_id_impl_tm_notin_syms
+          uniformize_fun.simps(2) verit_comp_simplify1(3))
+    finally show ?thesis .
+  next
+    case unif
+    hence unif_ite: "replace_tm t A r = r \<or> length r < 2" using tm_notin_syms_impl_replace_tm_id 
+      by fast
+    with lr_def have "uniformize_fun t A (xs@ys) (p#ps) = uniformize_fun t A (xs@ys) ps" 
+      by fastforce
+    also have "... = xs @ uniformize_fun t A ys ps" using Cons .
+    also have "... = xs @ uniformize_fun t A ys (p#ps)" using unif_ite lr_def by fastforce
+    finally show ?thesis .
+  qed
+qed simp
+  
+
+lemma uniformize_fun_neq_ps0_impl_uniformized:
+  assumes "uniformize_fun t A ps0 ps \<noteq> ps0"
+  obtains l r q s where "(l,r) \<in> set ps"
+                    "r \<noteq> replace_tm t A r"
+                    "length r \<ge> 2"
+                    "ps = q@[(l,r)]@s"
+                    "\<forall>(l,r)\<in>set q. length r < 2 \<or> Tm t \<notin> set r"
+using assms proof (induction ps arbitrary: thesis)
+  case (Cons p ps)
+  obtain l0 r0 where lr0_def: "p = (l0,r0)" by fastforce
+  consider (not_fst) "length r0 < 2 \<or> Tm t \<notin> set r0" | (fst) "length r0 \<ge> 2 \<and> Tm t \<in> set r0" 
+    by linarith
+  then show ?case 
+  proof cases
+    case not_fst
+    hence "uniformize_fun t A ps0 (p#ps) = uniformize_fun t A ps0 ps"
+      using lr0_def tm_notin_syms_impl_replace_tm_id by fastforce
+    then obtain l r q s where lrqs_defs: 
+                              "(l,r) \<in> set ps"
+                              "r \<noteq> replace_tm t A r"
+                              "length r \<ge> 2"
+                              "ps = q@[(l,r)]@s"
+                              "\<forall>(l,r)\<in>set q. length r < 2 \<or> Tm t \<notin> set r"
+      using Cons(1,3) by (metis (lifting))
+    moreover from this not_fst lr0_def have 
+                               "(l,r) \<in> set (p#ps)" "p#ps = (p#q)@[(l,r)]@s"
+                               "\<forall>(l,r)\<in> set (p#q). length r < 2 \<or> Tm t \<notin> set r"
+      by simp+
+    ultimately show ?thesis using Cons(2) by blast
+  next
+    case fst
+    hence "r0 \<noteq> replace_tm t A r0" find_theorems name:replace_tm
+      using replace_tm_id_impl_tm_notin_syms by metis
+    with fst lr0_def show ?thesis using Cons(2)[of _ _ "[]"] by simp
+  qed
+qed simp
+
+  
+
+lemma uniformize_fun_uniformizes_fst:
+  assumes "(l,r) \<in> set ps"
+          "r \<noteq> replace_tm t A r"
+          "ps = q@[(l,r)]@s"
+          "\<forall>(l,r)\<in>set q. Tm t \<notin> set r \<or> length r < 2"
+          "length r \<ge> 2"
+          "A = fresh (nts ps)"
+        shows
+    "uniformize_fun t A ps ps = ((removeAll (l,r) ps) @ [(A, [Tm t]), (l, replace_tm t A r)])" 
+proof -
+  from assms(3,4) uniformize_fun_ps0_app[OF assms(6)] 
+      uniformize_fun_uniform_prepend have
+    "uniformize_fun t A ps ps = q @ uniformize_fun t A ([(l,r)]@s) ([(l,r)]@s)" by fastforce
+  also have "... = q @ (removeAll (l,r) ([(l,r)]@s)) @ [(A, [Tm t]), (l, replace_tm t A r)]"
+    using assms(2,5) by fastforce
+  also have "... = removeAll (l,r) ps @ [(A, [Tm t]), (l, replace_tm t A r)]"
+  proof -
+    have "(l,r) \<notin> set q" 
+      using assms(2,4,5) tm_notin_syms_impl_replace_tm_id by fastforce 
+    thus ?thesis using assms(3) by simp
+  qed
+  finally show ?thesis .
+qed
+
+lemma uniformize_single_is_uniformized:
+  assumes "uniformize_fun t A ps ps \<noteq> ps"
+          "A = fresh (nts ps \<union> {S})"
+  shows "uniformize A t S ps (uniformize_fun t A ps ps)"
+proof -
+  from assms obtain l r q s  where lr_in_ps: "(l,r) \<in> set ps"
+                          and replace_neq: "r \<noteq> replace_tm t A r"
+                          and len_lb: "length r \<ge> 2"
+                          and ps_qs: "ps = q@[(l,r)]@s"
+                          and q_uniform: "\<forall>(l,r)\<in>set q. length r < 2 \<or> Tm t \<notin> set r"
+    using uniformize_fun_neq_ps0_impl_uniformized 
+    by (smt (verit, del_insts) case_prodI2 case_prod_conv)
+  moreover obtain p s' where "r = p@[Tm t]@s'"
+                        and replace_eq_p_Nt_s: "replace_tm t A r = p@[Nt A]@s'"
+                        and "p \<noteq> [] \<or> s' \<noteq> []"
+  proof -
+    from replace_tm_replaces_single replace_neq obtain p s' where
+      "r = p@[Tm t]@s'"
+      "replace_tm t A r = p@[Nt A]@s'"
+      by metis
+    with len_lb show thesis using that by fastforce
+  qed
+  moreover have "uniformize_fun t A ps ps = removeAll (l,r) ps @ [(A, [Tm t]), (l, p @ [Nt A] @ s')]" 
+  proof -
+    have fresh_A: "A = fresh (nts ps)" using assms(2) 
+      sorry
+    with uniformize_fun_uniformizes_fst[OF lr_in_ps replace_neq ps_qs _ len_lb fresh_A] 
+     show ?thesis using replace_eq_p_Nt_s q_uniform by auto
+  qed
+  ultimately show ?thesis
+    unfolding uniformize_def using assms by blast
+qed
+
+
+  
+
 
 
 
